iqsort test definition

example_array.v
@@ -14,7 +14,7 @@ Unset Strict Implicit.
 Unset Printing Implicit Defensive.
 
 Local Open Scope order_scope.
-Import Order.TTheory.
+Import Order.Theory.
 Local Open Scope monae_scope.
 Local Open Scope tuple_ext_scope.
 
@@ -22,8 +22,10 @@ From infotheo Require Import ssrZ.
 Require Import ZArith.
 
 Section marray.
-Variables (E : UU0) (M : arrayMonad E Z_eqType).
-Variables (d : unit) (T : porderType d).
+(* Variables (E : UU0) (M : arrayMonad E Z_eqType).
+Variables (d : unit) (T : porderType d). *)
+
+Variable (d : unit) (E : porderType d) (M : arrayMonad E Z_eqType).
 
 Fixpoint readList (i : Z) (n : nat) : M (seq E) :=
   if n isn't k.+1 then Ret [::] else liftM2 cons (aget i) (readList (i + 1) k).
@@ -40,27 +42,31 @@ Definition write3L (i : Z) '(xs, ys, zs) :=
   writeList i (xs ++ ys ++ zs) >> Ret (size xs, size ys, size zs).
 
 Definition swap (i j : Z) : M unit := 
-  aGet i >>= (fun x => aGet j >>= (fun y => aPut i y >> aPut j x)).
+  aget i >>= (fun x => aget j >>= (fun y => aput i y >> aput j x)).
 
-Fixpoint partl (p : T) (s : (seq T * seq T)%type) (xs : seq T): (seq T * seq T)%type :=
+Fixpoint partl (p : E) (s : (seq E * seq E)%type) (xs : seq E): (seq E * seq E)%type :=
   match xs with
   | [::] => s
   | x :: xs => if x <= p then partl p (s.1 ++ [:: x], s.2) xs
-                                   else partl p (s.1, s.2 ++ [:: x]) xs
+                         else partl p (s.1, s.2 ++ [:: x]) xs
   end.
 
 Definition second {A B C} (f : B -> M C) (xy : (A * B)%type) := f xy.2 >>= (fun y' => Ret (xy.1, y')).
 
-Program Fixpoint partl' (p : T) (s : (seq T * seq T)) (xs : seq T): M (seq T * seq T)%type :=
-  match xs with
-  | [::] => Ret s
-  | x :: xs => if x <= p then qperm s.2 >>= (fun zs' => partl' p (s.1 ++ [:: x], s.2) xs)
-                         else partl' p (s.1, s.2 ++ [:: x]) xs
-  end.
+(* Program Fixpoint partl' (p : E) (s : (seq E * seq E * seq E)) : M (seq E * seq E)%type :=
+  match s with
+  | (ys, zs, [::]) => Ret (ys, zs)
+  | (ys, zs, x :: xs) => if x <= p then (@qperm _ _ zs) >>= (fun zs' => partl' p (ys ++ [:: x], zs', xs))
+                         else partl' p (ys, zs ++ [:: x], xs)
+  end. *)
 
-Lemma ipartl_spec (i : Z) (p : E) (ys zs xs : seq E) (ipartl : E -> Z -> (nat * nat * nat)%type -> M (nat * nat)%type): 
+(* Definition dispatch (x p : E) '(ys, zs, xs) := 
+  if x <= p then perm zs >>= (fun zs' => Ret (ys ++ [:: x], zs', xs))
+            else perm (zs ++ [:: x]) >>= (fun zs' => Ret (ys, zs', zs)). *)
+
+(* Lemma ipartl_spec (i : Z) (p : E) (ys zs xs : seq E) (ipartl : E -> Z -> (nat * nat * nat)%type -> M (nat * nat)%type): 
   writeList i (ys ++ zs ++ xs) >> ipartl p i (size ys, size zs, size xs)
-    `<=` second perm (partl p (ys, zs) xs) >>= write2L i.
+    `<=` second perm (partl p (ys, zs) xs) >>= write2L i. *)
 
 Local Open Scope zarith_ext_scope.
 
@@ -71,4 +77,34 @@ elim: xs i => [|h t ih] i /=; first by rewrite bindretf addZ0.
 by rewrite ih bindA -addZA add1Z natZS.
 Qed.
 
+Fixpoint ipartl (p : E) (i : Z) (ny nz : nat) (nx : nat) : M (nat * nat)%type := 
+  match nx with
+  | 0 => Ret (ny, nz)
+  | k.+1 => aget ((* i + *) (ny + nz)%:Z) >>= (fun x => (* TODO *)
+         if x <= p then swap (i + ny%:Z) (i + ny%:Z + nz%:Z) >> ipartl p i (ny + 1) nz k
+                   else ipartl p i ny (nz.+1) k)
+  end.
+
+(* Program Fixpoint iqsort (i : Z) (n : nat) : M unit := 
+  match n with
+  | 0 => Ret tt
+  | n.+1 => aget i >>= (fun p =>
+         ipartl p (i) 0 0 n >>= (fun '(ny, nz) =>
+         swap i (i + ny%:Z) >>
+         iqsort i ny >> iqsort (ny%:Z) nz))
+  end. *)
+
+(* Lemma lemma12 {i : Z} {xs : seq E} {p : E} : 
+  writeList i xs >> iqsort i (size xs) `<=` _.
+Proof. *)
+
+(* Lemma lemma13 {i : Z} {ys : seq E} {p : E} : 
+  perm ys >>= (fun ys' => writeList i (ys' ++ [:: p])) `>=` 
+  writeList i (p :: ys) >> swap i (i + (size ys)%:Z).
+Proof. *)
+  
+(* Qed. *)
+
 End marray.
+
+
